##################
The angle sum rule
##################

The angle sum rule is:

.. math::

    \sin(\alpha \pm \beta) = \sin \alpha \cos \beta \pm \cos \alpha \sin \beta

    \cos(\alpha \pm \beta) = \cos \alpha \cos \beta \mp \sin \alpha \sin \beta

*****
Proof
*****

Let's say we have a vector $(x_1, y_1)$ resulting from the anticlockwise
rotation of a length 1 vector $(1, 0)$ by $\alpha$ degrees around the origin.

We rotate this vector another $\beta$ degrees anticlockwise around the origin
to give length 1 vector $(x_2, y_2)$.

.. image:: images/angle_sum.png

We can see from the picture that:

.. math::

    \cos(\alpha + \beta) = x_2 = r - u

    \sin(\alpha + \beta) = y_2 = t + s

We are going to use some basic trigonometry to get the lengths of $r, u, t,
s$.

Because the angles in a triangle sum to 180 degrees, $\phi$ on the picture is
$90 - \alpha$ and therefore the angle between lines $q, t$ is also $\alpha$.

Remembering the definitions of $\cos$ and $\sin$:

.. math::

    \cos\theta = \frac{A}{H} \implies A = (\cos \theta) H

    \sin\theta = \frac{O}{H} \implies O = (\sin \theta) H

Thus:

.. math::

    p = \cos \beta

    q = \sin \beta

    r = (\cos \alpha) p = \cos \alpha \cos \beta

    s = (\sin \alpha) p = \sin \alpha \cos \beta

    t = (\cos \alpha) q = \cos \alpha \sin \beta

    u = (\sin \alpha) q = \sin \alpha \sin \beta

So:

.. math::

    \cos(\alpha + \beta) = x_2 = r - u = \cos \alpha \cos \beta - \sin \alpha \sin
    \beta

    \sin(\alpha + \beta) = y_2 = t + s = \sin \alpha \cos \beta + \cos \alpha \sin \beta


.. include:: links_names.inc
